theories/Symbolic/Sound.v
@@ -2008,10 +2008,8 @@ Module Soundness
     unfold SMut.ValidContract, CMut.ValidContract, ForallNamed.
     rewrite Forall_forall. intros [Hwp] ι.
     unfold SMut.exec_contract_path in Hwp.
-    (* rewrite prune_sound in Hwp. *)
-    (* rewrite Experimental.solve_uvars_sound in Hwp. *)
-    (* specialize (Hwp env_nil). *)
-    inster Hwp by reflexivity.
+    rewrite Postprocessing.prune_sound in Hwp.
+    rewrite Postprocessing.solve_uvars_sound in Hwp.
     rewrite Postprocessing.prune_sound in Hwp.
     rewrite Postprocessing.solve_evars_sound in Hwp.
     rewrite Postprocessing.prune_sound in Hwp. cbn in Hwp.
@@ -2023,24 +2021,5 @@ Module Soundness
   Qed.
 
   (* Print Assumptions symbolic_sound. *)
-
-  Lemma symbolic_sound_solve_uvars {Γ τ} (c : SepContract Γ τ) (body : Stm Γ τ) :
-    SMut.ValidContractSolveUVars c body ->
-    CMut.ValidContract c body.
-  Proof.
-    unfold SMut.ValidContract, CMut.ValidContract, ForallNamed.
-    rewrite Forall_forall. intros [Hwp] ι.
-    unfold SMut.exec_contract_path in Hwp.
-    rewrite Postprocessing.prune_sound in Hwp.
-    rewrite Postprocessing.solve_uvars_sound in Hwp.
-    rewrite Postprocessing.prune_sound in Hwp.
-    rewrite Postprocessing.solve_evars_sound in Hwp.
-    rewrite Postprocessing.prune_sound in Hwp.
-    apply safe_demonic_close with _ ι in Hwp. revert Hwp.
-    rewrite <- (wsafe_safe (w := @MkWorld (sep_contract_logic_variables c) nil)).
-    apply approx_exec_contract; auto.
-    intros w1 ω01 ι1 -> Hpc1.
-    auto.
-  Qed.
 
 End Soundness.
